work on indexing

src/indexing.v
@@ -10,10 +10,25 @@ From stdpp Require Import list.
 Require Import Burrow.gmap_utils.
 Require Import Burrow.rollup.
 
+Definition PathLoc := list nat.
+
 Context {M: Type} `{!EqDecision M, !TPCM M} `{!Countable M}.
 Context `{!EqDecision RefinementIndex}.
 Context {refinement_of_index : RefinementIndex -> Refinement M M}.
 
-Definition PathLoc := list nat.
+Definition node_of_pl (node: Node M) (pl: PathLoc) : Node M. Admitted.
+Definition every_node (node: Node M) (fn : Node M -> Prop) : Prop. Admitted.
 
-Definition node_of_pl (node: Node M) (pl: PathLoc) : Node M.
+Lemma every_node_equiv_forall
+    (node : Node M) (fn : Node M -> Prop) (rtriv: ∀ n , node_trivial n -> fn n)
+  : (every_node node fn) <-> (forall pl , fn (node_of_pl node pl)). Admitted.
+
+Lemma forall_node_op
+    (node1 : Node M) (node2 : Node M)
+  : forall pl , (node_of_pl node1 pl) ⋅ (node_of_pl node2 pl) ≡ node_of_pl (node1 ⋅ node2) pl.
+Admitted.
+
+Lemma equiv_existentiality_cells
+    (node1 : Node M) (node2 : Node M)
+  : forall pl , (node_of_pl node
+  
